

Q6. In class, we talked about how to compute the sample mean of a variable X .

$$m(X) = \frac{1}{N} \sum_{i=1}^N x_i$$

and sample covariance of two variables X and Y ,

$$\text{cov}(X, Y) = \frac{1}{N} \sum_{i=1}^N (x_i - m(X))(y_i - m(Y)).$$

Recall, the sample variance of X is

$$s^2 = \frac{1}{N} \sum_{i=1}^N (x_i - m(X))^2.$$

It can be very helpful to understand some basic properties of these statistics. If you want to write your calculations on a piece of paper, take a photo, and upload that to your GitHub repo, that's probably easiest.

We're going to look at **linear transformations** of X , $Y = a + bX$. So we take each value of X , x_i , and transform it as $y_i = a + bx_i$.

1. Show that $m(a + bX) = a + b \cdot m(X)$.

2. Show that $\text{cov}(X, X) = s^2$.

3. Show that $\text{cov}(X, a + bY) = b \cdot \text{cov}(X, Y)$.

4. Show that $\text{cov}(a + bX, a + bY) = b^2 \text{cov}(X, Y)$. Notice, this also means that $\text{cov}(bX, bX) = b^2 s^2$.

5. Suppose $b > 0$ and let the median of X be $\text{med}(X)$. Is it true that the median of $a + bX$ is equal to $a + b \cdot \text{med}(X)$? Is the IQR of $a + bX$ equal to $a + b \cdot \text{IQR}(X)$?

6. Show by example that the means of X^2 and \sqrt{X} are generally not $(m(X))^2$ and $\sqrt{m(X)}$. So, the results we derived above really depend on the linearity of the transformation $Y = a + bX$, and transformations like $Y = X^2$ or $Y = \sqrt{X}$ will not behave in a similar way.

Transformed variable

1) $Y = a + bX \rightarrow y_i = a + bx_i$

Sample mean of Y

$$m(Y) = \frac{1}{N} \sum_{i=1}^N y_i$$

$$m(Y) = \frac{1}{N} \sum_{i=1}^N (a + bx_i)$$

$$= \frac{1}{N} \left(a \sum_{i=1}^N 1 + b \sum_{i=1}^N x_i \right)$$

$$= \frac{1}{N} \left(aN + b \sum_{i=1}^N x_i \right)$$

$$= a + b \cdot \frac{1}{N} \sum_{i=1}^N x_i$$

$$m(Y) = a + b m(X)$$

2) $Y = X$ in covariance formula

$$\text{cov}(X, X) = \frac{1}{N} \sum_{i=1}^N (x_i - m(X))(x_i - m(X))$$

$$\text{cov}(X, X) = \frac{1}{N} \sum_{i=1}^N (x_i - m(X))^2$$

$$s^2 = \frac{1}{N} \sum_{i=1}^N (x_i - m(X))^2 \quad \text{so} \quad \text{cov}(X, X) = s^2$$

3) covariance formula

$$\text{cov}(X, Z) = \frac{1}{N} \sum_{i=1}^N (x_i - m(X))(z_i - m(Z))$$

linear transformation

$$Z = a + bY \rightarrow z_i = a + by_i$$

Sample mean

$$m(Z) = a + b m(Y)$$

$$\text{cov}(X, a + bY) = \frac{1}{N} \sum_{i=1}^N (x_i - m(X))(a + by_i - m(a + bY))$$

$$= \frac{1}{N} \sum_{i=1}^N (x_i - m(X)) b (y_i - m(Y))$$

$$\text{cov}(X, a + bY) = b \cdot \frac{1}{N} \sum_{i=1}^N (x_i - m(X))(y_i - m(Y))$$

$$\text{so} \quad \text{cov}(X, a + bY) = b \cdot \text{cov}(X, Y)$$

4) Substitute bX into covariance formula

$$\text{cov}(bX, bX) = \frac{1}{N} \sum_{i=1}^N (bx_i - m(bX))(bx_i - m(bX))$$

From part 1: $m(bX) \rightarrow b m(X)$

$$\text{cov}(bX, bX) = \frac{1}{N} \sum_{i=1}^N (bx_i - b m(X))(bx_i - b m(X))$$

$$= \frac{1}{N} \sum_{i=1}^N (b(x_i - m(X)))(b(x_i - m(X)))$$

$$= \frac{1}{N} \sum_{i=1}^N b^2 (x_i - m(x))^2$$

$$\text{Cov}(bX, bX) = b^2 \frac{1}{N} \sum_{i=1}^N (x_i - m(x))^2$$

$$s^2 = \frac{1}{N} \sum_{i=1}^N (x_i - m(x))^2 \quad \text{so} \quad \text{cov}(bX, bX) = b^2 s^2$$

5) Given: $Y = a + bX$, $b > 0$

Median

half of the $x_i \leq \text{med}(x)$, half of the $x_i \geq \text{med}(x)$

Since $b > 0$ order is the same

$$x_i \leq \text{med}(x) \rightarrow a + bx_i \leq a + b\text{med}(x)$$

$$x_i \geq \text{med}(x) \rightarrow a + bx_i \geq a + b\text{med}(x)$$

so median of Y is: $\text{med}(Y) = \text{med}(a + bX) = a + b\text{med}(x)$

IQR

75% of the $x_i \leq Q3_x$

$$\text{IQR} = Q3_x - Q1_x \rightarrow 25\% \text{ of the } x_i \leq Q1_x$$

linear transformation

$$\text{if } x_i \leq Q1_x, \text{ then } a + bx_i \leq a + bQ1_x$$

$$\text{if } x_i \leq Q3_x, \text{ then } a + bx_i \leq a + bQ3_x$$

so exactly the same 25% of observations that were below $Q1_x$ in X are below $a + bQ1_x$ in Y

$$Q1_y = a + bQ1_x, \quad Q3_y = a + bQ3_x$$

compute IQR

$$\text{IQR}(Y) = Q3_y - Q1_y = (a + bQ3_x) - (a + bQ1_x) = b(Q3_x - Q1_x) = b\text{IQR}(x)$$

$$\rightarrow \text{IQR}(a + bX) = b\text{IQR}(x) \neq a + b\text{IQR}(x)$$

6)

Example mean

$$m(x) = \frac{1+3}{2} = 2$$

mean of x^2

$$x^2 = \{1^2, 3^2\} = \{1, 9\}$$

$$m(x^2) = \frac{1+9}{2} = 5$$

$$(m(x))^2 = 2^2 = 4$$

$$\rightarrow m(x^2) \neq (m(x))^2$$

mean of \sqrt{x}

$$\sqrt{x} = \{\sqrt{1}, \sqrt{3}\}$$

$$m(\sqrt{x}) = \frac{\sqrt{1} + \sqrt{3}}{2}$$

$$\rightarrow m(\sqrt{x}) \neq \sqrt{m(x)}$$

$$\sqrt{m(x)} = \sqrt{2}$$